$$f(x) = 
\begin{cases}
\cos x & \text{si } \text{ } x \leq 0\\
-x^2+a  & \text{si } \text{ } x > 0
\end{cases}
$$

\\matrix
$$A = 
\begin{pmatrix}
x & x+1 \\
x^{2}+x+1 & x^{2}
\end{pmatrix}
$$


$$
\begin{vmatrix} 
-1 & 2\\
\frac{1}{2} & -1\\
\end{vmatrix}=0 
$$

//Gauss - Jordan
$$
\begin{pmatrix}
\begin{array}{ccc|ccc}
-1 & 2 & 0 &1&0&0\\
0 & 1 & -2 &0&1&0\\
3&5&3&0&0&1\\
\end{array} 
\end{pmatrix}

\xrightarrow{F1=-F1}

\begin{pmatrix}
\begin{array}{ccc|ccc}
1 & -2 & 0 &-1&0&0\\
0 & 1 & -2 &0&1&0\\
3&5&3&0&0&1\\
\end{array} 
\end{pmatrix}


\xrightarrow{F3=3F1-F3}

\begin{pmatrix}
\begin{array}{ccc|ccc}
1 & -2 & 0 &-1&0&0\\
0 & 1 & -2 &0&1&0\\
0&-11&-3&-3&0&-1\\
\end{array} 
\end{pmatrix}



//sistemes d'equacions
\left. 

\begin{array}{rcl} 
y+(\lambda-1)z& = & \lambda \\ 
(\lambda-1)y +z& = & \lambda \\ 
(\lambda-2)x & = & \lambda+2
\end{array} 

\right\}


//inversa de una matriz por adjuntos

$$A^{-1} =\frac{1}{det(A)}·(AdjA)^t=\frac{1}{1} · 
\begin{pmatrix}
\begin{vmatrix} 
1 & 1\\
0 & 1\\
\end{vmatrix}&&

-\begin{vmatrix} 
0 & 1\\
0 & 1\\
\end{vmatrix}&&

\begin{vmatrix} 
0 & 1\\
0 & 0\\
\end{vmatrix}&&
\\


-\begin{vmatrix} 
1 & 1\\
0 & 1\\
\end{vmatrix}&&

\begin{vmatrix} 
1 & 1\\
0 & 1\\
\end{vmatrix}&&

-\begin{vmatrix} 
1 & 1\\
0 & 0\\
\end{vmatrix}&&
\\


\begin{vmatrix} 
1 & 1\\
1 & 1\\
\end{vmatrix}&&

-\begin{vmatrix} 
1 & 1\\
0 & 1\\
\end{vmatrix}&&

\begin{vmatrix} 
1 & 1\\
0 & 0\\
\end{vmatrix}&&
\\

\end{pmatrix}^t

=

\begin{pmatrix}
1&&-1&&0\\
0&&1&&-1\\
0&&0&&1
\end{pmatrix}
$$





$$
